tools/Vale/src/emit_common_quick_code.fs
@@ -11,7 +11,83 @@ open Emit_common_base
 open Microsoft.FSharp.Math
 open System.Numerics
 
-let build_qcode (env:env) (loc:loc) (p:proc_decl):decls =
+let rec build_qcode_stmt (s:stmt):exp =
+  let err () = internalErr "make_gen_quick_block" in
+  match skip_loc_stmt s with
+  | SAssign ([], e) ->
+    (
+      match skip_loc e with
+      | EApply(Id x, es) ->
+          let es = List.filter (fun e -> match e with EOp (Uop UGhostOnly, _) -> false | _ -> true) es in
+          let es = List.map get_code_exp es in
+          let es = List.map (map_exp stateToOp) es in
+          let es = List.map exp_refined es in
+          vaApp ("quick_" + x) es
+      | _ -> err ()
+    )
+  | _ -> err ()
+and build_qcode_stmts (ss:stmt list):exp =
+  let empty = EApply (Id "QEmpty", []) in
+  let cons el e = EApply (Id "QSeq", [e; el]) in
+  List.fold cons empty (List.rev (List.map build_qcode_stmt ss))
+and build_qcode_block (ss:stmt list):exp =
+  EApply (Id "qblock", [build_qcode_stmts ss])
+
+let make_gen_quick_block (loc:loc) (p:proc_decl):((env -> quick_info -> lhs list -> exp list -> stmt list -> stmt list) * (unit -> decls)) =
+  let funs = ref ([]:decls) in
+  let fArgs = (List.collect fArg p.prets) @ (List.collect fArg p.pargs) in
+  let fParams = make_fun_params p.prets p.pargs in
+  let gen_quick_block env info outs args ss =
+    let id = Reserved ("qcode_" + info.qsym + "_" + (string_of_id p.pname)) in
+    let cid = Reserved ("code_" + info.qsym + "_" + (string_of_id p.pname)) in
+    let tArgs = List.map (fun (x, _) -> TName x) fParams in
+    let tCodeApp = TApp (TName cid, tArgs) in
+//    let fBody = build_qcode_block ss in
+    let fBody = build_qcode_stmts ss in
+    let fCode =
+      {
+        fname = id;
+        fghost = Ghost;
+        fargs = fParams;
+//        fret = TApp (TName (Reserved "quickCode"), [TName (Id "unit"); tCodeApp]);
+        fret = TApp (TName (Id "quickCodes"), [TName (Id "unit"); tCodeApp]);
+        fbody = Some fBody;
+        fattrs = [(Id "opaque_to_smt", [])];
+      }
+      in
+    let dFun = DFun fCode in
+    funs := (loc, dFun)::!funs;
+    (*
+      let (va_s2, va_fc2, ()) = wp_run_code_norm (va_code_1_Incr3 ()) (va_quick_1_Incr3 ()) va_s0
+        (fun (s0:state) (sN:state) -> va_update_reg Rax sN (va_update_flags sN s0))
+        (fun (sN:state) (sN':state) -> va_get_reg Rax sN == va_get_reg Rax sN' /\ va_get_flags sN == va_get_flags sN')
+    *)
+    let eCode = EApply (cid, fArgs) in
+    let eQCode = EApply (id, fArgs) in
+    let s0 = Reserved "s0" in
+    let sM = Reserved "sM" in
+    let sN = Reserved "sN" in
+    let eqMod x =
+      let getM = stateGet {env with state = EVar sM} x in
+      let getN = stateGet {env with state = EVar sN} x in
+      EOp (Bop BEq, [getM; getN])
+      in
+    let eEq = and_of_list (List.map eqMod info.qmods) in
+    let fEq = EBind (Lambda, [], [(sM, Some tState); (sN, Some tState)], [], eEq) in
+    let frameMod e x =
+      match Map.tryFind x env.ids with
+      | Some (StateInfo (prefix, es, t)) -> vaApp ("update_" + prefix) (es @ [EVar sN; e])
+      | _ -> internalErr ("gen_quick_block: could not find variable " + (err_id x))
+      in
+    let eUpdate = List.fold frameMod (EVar s0) info.qmods in
+    let fUpdate = EBind (Lambda, [], [(s0, Some tState); (sN, Some tState)], [], eUpdate) in
+    let sLemma = SAssign (outs, EApply (Id "wp_run_norm", eCode::eQCode::args @ [fUpdate; fEq])) in
+    [sLemma]
+    in
+  let gen_quick_block_funs () = List.rev !funs in
+  (gen_quick_block, gen_quick_block_funs)
+
+let build_qcode (env:env) (loc:loc) (p:proc_decl) (ss:stmt list):decls =
   (*
   [@"opaque_to_smt"]
   let va_qcode_Add3 () : quickCode unit (va_code_Add3 ()) = qblock (
@@ -23,8 +99,11 @@ let build_qcode (env:env) (loc:loc) (p:proc_decl):decls =
   )
   *)
   let fParams = [] in
-  let tRetQuick = TApp (TName (Id "quickCode"), []) in
-  let eQuick = EApply (Id "QEmpty", []) in
+  let cid = Reserved ("code_" + (string_of_id p.pname)) in
+  let tArgs = List.map (fun (x, _) -> TName x) fParams in
+  let tCodeApp = TApp (TName cid, tArgs) in
+  let tRetQuick = TApp (TName (Id "quickCode"), [TName (Id "unit"); tCodeApp]) in
+  let eQuick = build_qcode_block ss in
   let fCodes =
     {
       fname = Reserved ("qcode_" + (string_of_id p.pname));
@@ -46,7 +125,8 @@ let build_proc_body (env:env) (loc:loc) (p:proc_decl) (code:exp) (ens:exp):stmt 
   let fM = Reserved "fM" in
   let sM = Reserved "sM" in
   let g = Reserved "g" in
-  let wpSound_X = Reserved ("wpSound_" + (string_of_id p.pname)) in
+//  let wpSound_X = Reserved ("wpSound_" + (string_of_id p.pname)) in
+  let wpSound_X = Id "wp_sound_code_norm" in
   let qCodes_X = Reserved ("qcode_" + (string_of_id p.pname)) in
   let ghostRets = List.collect (fun (x, t, g, _, _) -> match g with XGhost -> [(x, t)] | _ -> []) p.prets in
   let gAssigns = List.map (fun (x, _) -> (x, None)) ghostRets in
